aeq.compose, change aeq to use exp in type
Change other theorems to use new aeq.

aeq.lean
@@ -4,56 +4,56 @@ import exp
 
 open nat
 open set
-
-inductive aeq₁ : set (ℕ × ℕ)  → Type :=
-  | var : Π R    x y, (x, y) ∈ R                → aeq₁ R
-  | app : Π {R}     , aeq₁ R → aeq₁ R           → aeq₁ R
-  | lam : Π {R}  x y, aeq₁ (symm_update₁ R x y) → aeq₁ R
-
-inductive aeq₂ : Π (X : set ℕ) (Y : set ℕ), sset X Y → Type :=
-  | var : Π {X Y R} x y, sset.mem x y R                                     → aeq₂ X Y R
-  | app : Π {X Y R}    , aeq₂ X Y R → aeq₂ X Y R                            → aeq₂ X Y R
-  | lam : Π {X Y R} x y, aeq₂ (insert x X) (insert y Y) (symm_update R x y) → aeq₂ X Y R
-
 open sset
 open exp₂
-open aeq₂
 
-definition map_aeq₂
-: ∀{X Y X' Y'} {R : sset X Y} {S : sset X' Y'}
+inductive aeq : Π{X Y}, sset X Y → exp₂ X → exp₂ Y → Type :=
+  | var : Π{X Y} {R : sset X Y} x y (m : sset.mem x y R),                                                              aeq R (var x (mem_left m)) (var y (mem_right m))
+  | app : Π{X Y} {R : sset X Y} {f₁ e₁ : exp₂ X} {f₂ e₂ : exp₂ Y}, aeq R f₁ f₂ → aeq R e₁ e₂                         → aeq R (app f₁ e₁)          (app f₂ e₂)
+  | lam : Π{X Y} {R : sset X Y} x y {e₁ : exp₂ (insert x X)} {e₂ : exp₂ (insert y Y)}, aeq (symm_update R x y) e₁ e₂ → aeq R (lam x e₁)           (lam y e₂)
+
+open aeq
+
+definition aeq_left  {X Y} {R : sset X Y} {e₁ e₂} : aeq R e₁ e₂ → exp₂ X := λ a, e₁
+definition aeq_right {X Y} {R : sset X Y} {e₁ e₂} : aeq R e₁ e₂ → exp₂ Y := λ a, e₂
+
+definition aeq.map
+: ∀{X Y} {R : sset X Y} {S : sset X Y} {e₁ : exp₂ X} {e₂ : exp₂ Y}
 , (∀{x y}, mem x y R → mem x y S)
-→ aeq₂ X Y R
-→ aeq₂ X' Y' S
-  | X Y X' Y' R S f (var x y x_y_mem_R) := var x y (@f x y x_y_mem_R)
-  | X Y X' Y' R S f (app e₁ e₂)         := app (map_aeq₂ f e₁) (map_aeq₂ f e₂)
-  | X Y X' Y' R S f (lam x y e)         :=
+→ aeq R e₁ e₂ → aeq S e₁ e₂
+  | X Y R S (var x x_mem_X) (var y y_mem_Y) f (var x y x_y_mem_R) := var x y (@f x y x_y_mem_R)
+  | X Y R S (app f₁ e₁)     (app f₂ e₂)     f (app a₁ a₂)         := app (aeq.map f a₁) (aeq.map f a₂)
+  | X Y R S (lam x e₁)      (lam y e₂)      f (lam x y a)         :=
     have f' : ∀ a b, mem a b (symm_update R x y) → mem a b (symm_update S x y), from
       λ a b, map_symm_update f,
-    lam x y (map_aeq₂ f' e)
+    lam x y (aeq.map f' a)
 
-theorem aeq_id : ∀{X}, exp₂ X → aeq₂ X X (id X)
+theorem aeq.id : ∀{X} (e : exp₂ X), aeq (id X) e e
   | X (var x x_mem_X) := var x x (and.intro x_mem_X (and.intro x_mem_X (and.intro rfl x_mem_X)))
-  | X (app e₁ e₂)     := app (aeq_id e₁) (aeq_id e₂)
+  | X (app e₁ e₂)     := app (aeq.id e₁) (aeq.id e₂)
   | X (lam x e)       :=
     have f : ∀ a b, mem a b (id (insert x X)) → mem a b (symm_update (id X) x x), from
       λ a b, iff.elim_right mem_symm_update_id,
-    lam x x (map_aeq₂ f (aeq_id e))
+    lam x x (aeq.map f (aeq.id e))
 
-/-
-theorem aeq_id.right : ∀{X}, aeq₂ X X (id X) → exp₂ X
-  | X (@aeq₂.var _ _ (id X) x x x_x_mem_X) := var x (mem_left x_x_mem_X)
-  | X (app e₁ e₂)         := app (aeq_id.right e₁) (aeq_id.right e₂)
-  | X (lam x x e)         :=
-    have f : ∀ a b, mem a b (symm_update (id X) x x) → mem a b (id (insert x X)), from
-      λ a b, iff.elim_left mem_symm_update_id,
-    lam x (aeq_id.right (map_aeq₂ f e))
--/
-
-theorem aeq_inverse : ∀{X Y R}, aeq₂ X Y R → aeq₂ Y X (inverse R)
-  | X Y R (var x y x_y_mem_R) := var y x (mem_inverse x_y_mem_R)
-  | X Y R (app e₁ e₂)         := app (aeq_inverse e₁) (aeq_inverse e₂)
-  | X Y R (lam x y e)         :=
+theorem aeq.inverse : ∀{X Y} {R : sset X Y} {e₁ e₂}, aeq R e₁ e₂ → aeq (inverse R) e₂ e₁
+  | X Y R (var x x_mem_X) (var y y_mem_Y) (var x y x_y_mem_R) := var y x (mem_inverse x_y_mem_R)
+  | X Y R (app f₁ e₁)     (app f₂ e₂)     (app a₁ a₂)         := app (aeq.inverse a₁) (aeq.inverse a₂)
+  | X Y R (lam x e)       (lam y e₂)      (lam x y a)         :=
     have f : ∀ a b,  mem a b (inverse (symm_update R x y))
            → mem a b (symm_update (inverse R) y x), from
       λ a b, iff.elim_left mem_symm_update_inverse,
-    lam y x (map_aeq₂ f (aeq_inverse e))
+    lam y x (aeq.map f (aeq.inverse a))
+
+theorem aeq.compose
+: ∀{X Y Z} {R : sset X Y} {S : sset Y Z} {e₁ e₂ e₃}
+, aeq R e₁ e₂ → aeq S e₂ e₃ → aeq (compose R S) e₁ e₃
+  | X Y Z R S (var x x_mem_X) (var y y_mem_Y) (var z z_mem_Z) (var x y x_y_mem_R) (var y z y_z_mem_S) :=
+    var x z (iff.elim_left mem_compose (exists.intro y (and.intro x_y_mem_R y_z_mem_S)))
+  | X Y Z R S (app f₁ e₁)     (app f₂ e₂)     (app f₃ e₃)     (app a₁ a₂)         (app a₃ a₄)         :=
+    app (aeq.compose a₁ a₃) (aeq.compose a₂ a₄)
+  | X Y Z R S (lam x e)       (lam y e₂)      (lam z e₃)      (lam x y a₁)        (lam y z a₂)        :=
+    have f : ∀ a c, mem a c (compose (symm_update R x y) (symm_update S y z))
+           → mem a c (symm_update (compose R S) x z), from
+      λ a c, mem_symm_update_compose_of_mem_compose_symm_update,
+    lam x z (aeq.map f (aeq.compose a₁ a₂))
